generic/Zeta.Generic.Thread.fsti
@@ -22,7 +22,7 @@ let index #vspec (tl: vlog vspec) (i: seq_index tl) =
   let _, l = tl in
   S.index l i
 
-let prefix #vspec (tl: vlog vspec) (i: nat {i <= length tl}): vlog _ =
+let prefix_base #vspec (tl: vlog vspec) (i: nat {i <= length tl}): vlog _ =
   let tid, l = tl in
   tid, SA.prefix l i
 
@@ -37,8 +37,12 @@ let verifiable_log vspec = tl: vlog vspec { verifiable tl }
 (* if a thread log is verifiable, its prefix is verifiable *)
 val verifiable_implies_prefix_verifiable (#vspec:verifier_spec)
   (tl:verifiable_log vspec) (i:nat{i <= length tl}):
-  Lemma (ensures (verifiable (prefix tl i)))
-        [SMTPat (prefix tl i)]
+  Lemma (ensures (verifiable (prefix_base tl i)))
+        [SMTPat (prefix_base tl i)]
+
+let prefix #vspec (tl: verifiable_log vspec) (i: nat {i <= length tl})
+  : tl': verifiable_log _ {length tl' = i}
+  = prefix_base tl i
 
 (* the verifier state after processing a log *)
 let state #vspec (tl:verifiable_log vspec)
@@ -106,6 +110,37 @@ let is_blum_add_ep (#vspec:_) (ep: epoch) (tl: verifiable_log vspec) (i: seq_ind
   = is_blum_add tl i &&
     (let be = blum_add_elem tl i in be.t.e = ep)
 
+val add_seq (#vspec:_) (ep: epoch) (tl: verifiable_log vspec)
+  : S.seq (ms_hashfn_dom vspec.app)
+
+val add_seq_map (#vspec:_) (tl: verifiable_log vspec) (i: seq_index tl {is_blum_add tl i})
+  : (let be = blum_add_elem tl i in
+     let ep = be.t.e in
+     let as = add_seq ep tl in
+     j: SA.seq_index as { S.index as j = be })
+
+val add_seq_invmap (#vspec:_) (ep: epoch) (tl: verifiable_log vspec) (j: SA.seq_index (add_seq ep tl))
+  : i:seq_index tl { is_blum_add tl i /\ add_seq_map tl i = j  }
+
+val lemma_add_seq_map (#vspec:_) (tl: verifiable_log vspec) (i: seq_index tl {is_blum_add tl i})
+  : Lemma (ensures (let be = blum_add_elem tl i in
+                    let ep = be.t.e in
+                    let as = add_seq ep tl in
+                    let j = add_seq_map tl i in
+                    add_seq_invmap ep tl j = i))
+          [SMTPat (add_seq_map tl i)]
+
+val add_seq_map_monotonic (#vspec:_) (tl: verifiable_log vspec) (i1 i2: (i:seq_index tl {is_blum_add tl i}))
+  : Lemma (requires (let be1 = blum_add_elem tl i1 in
+                     let be2 = blum_add_elem tl i2 in
+                     be1.t.e = be2.t.e))
+          (ensures ((i1 <= i2 ==> add_seq_map tl i1 <= add_seq_map tl i2) /\
+                    (i2 <= i1 ==> add_seq_map tl i2 <= add_seq_map tl i1)))
+
+val add_seq_invmap_monotonic (#vspec:_) (ep: epoch) (tl: verifiable_log vspec) (j1 j2: SA.seq_index (add_seq ep tl))
+  : Lemma (ensures ((j1 <= j2 ==> add_seq_invmap ep tl j1 <= add_seq_invmap ep tl j2) /\
+                    (j2 <= j1 ==> add_seq_invmap ep tl j2 <= add_seq_invmap ep tl j1)))
+
 let is_blum_evict (#vspec:_) (tl: verifiable_log vspec) (i: seq_index tl)
   = GV.is_blum_evict (index tl i)
 
@@ -123,6 +158,40 @@ let is_blum_evict_ep (#vspec:_) (ep: epoch) (tl: verifiable_log vspec) (i: seq_i
   : bool
   = is_blum_evict tl i &&
     (let be = blum_evict_elem tl i in be.t.e = ep)
+
+val evict_seq (#vspec:_) (ep: epoch) (tl: verifiable_log vspec)
+  : S.seq (ms_hashfn_dom vspec.app)
+
+val evict_seq_map (#vspec:_) (tl: verifiable_log vspec) (i: seq_index tl {is_blum_evict tl i})
+  : (let be = blum_evict_elem tl i in
+     let ep = be.t.e in
+     let es = evict_seq ep tl in
+     j: SA.seq_index es { S.index es j = be })
+
+val evict_seq_invmap (#vspec:_) (ep: epoch) (tl: verifiable_log vspec) (j: SA.seq_index (evict_seq ep tl))
+  : i:seq_index tl { is_blum_evict tl i /\ evict_seq_map tl i = j  }
+
+val lemma_evict_seq_map (#vspec:_) (tl: verifiable_log vspec) (i: seq_index tl {is_blum_evict tl i})
+  : Lemma (ensures (let be = blum_evict_elem tl i in
+                    let ep = be.t.e in
+                    let as = evict_seq ep tl in
+                    let j = evict_seq_map tl i in
+                    evict_seq_invmap ep tl j = i))
+          [SMTPat (evict_seq_map tl i)]
+
+val evict_seq_map_monotonic (#vspec:_) (tl: verifiable_log vspec) (i1 i2: (i:seq_index tl {is_blum_evict tl i}))
+  : Lemma (requires (let be1 = blum_evict_elem tl i1 in
+                     let be2 = blum_evict_elem tl i2 in
+                     be1.t.e = be2.t.e))
+          (ensures ((i1 <= i2 ==> evict_seq_map tl i1 <= evict_seq_map tl i2) /\
+                    (i2 <= i1 ==> evict_seq_map tl i2 <= evict_seq_map tl i1)))
+
+val evict_seq_invmap_monotonic (#vspec:_) (ep: epoch) (tl: verifiable_log vspec) (j1 j2: SA.seq_index (evict_seq ep tl))
+  : Lemma (ensures ((j1 <= j2 ==> evict_seq_invmap ep tl j1 <= evict_seq_invmap ep tl j2) /\
+                    (j2 <= j1 ==> evict_seq_invmap ep tl j2 <= evict_seq_invmap ep tl j1)))
+
+val evict_elem_unique (#vspec:_) (tl: verifiable_log vspec) (i1 i2: (i: seq_index tl {is_blum_evict tl i}))
+  : Lemma (ensures (i1 <> i2 ==> blum_evict_elem tl i1 <> blum_evict_elem tl i2))
 
 (* is the i'th entry an app function *)
 let is_appfn (#vspec:_) (tl: verifiable_log vspec) (i: seq_index tl)
