generic/Zeta.Generic.Global.fst
@@ -5,14 +5,6 @@ let lemma_prefix_verifiable #vspec (gl: verifiable_log vspec) (i:nat{i <= S.leng
           [SMTPat (SA.prefix gl i)]
   = admit()
 
-let add_sseq (#vspec:_) (gl: verifiable_log vspec)
-  : ss:sseq (ms_hashfn_dom vspec.app) { S.length ss = S.length gl }
-  = admit()
-
-let evict_sseq (#vspec:_) (gl: verifiable_log vspec)
-  : ss:sseq (ms_hashfn_dom vspec.app) { S.length ss = S.length gl }
-  = admit()
-
 let app_fcrs
   (#vspec: verifier_spec)
   (gl: verifiable_log vspec): sseq (Zeta.AppSimulate.appfn_call_res vspec.app)
