utils/Zeta.SMap.fsti
@@ -1,0 +1,29 @@
+module Zeta.SMap
+
+open FStar.Seq
+open Zeta.SeqAux
+
+(* A mapping from one sequence to another *)
+let smap (#a:_) (s1 s2: seq a) = f:(seq_index s1 -> seq_index s2){
+  forall (i: seq_index s1). index s1 i == index s2 (f i)
+}
+
+(* injectivity property on smaps *)
+let into_prop (#a:Type) (#s1 #s2: seq a) (f:smap s1 s2)
+  = forall (i j: seq_index s1). (i <> j) ==> f i <> f j
+
+let into_smap (#a:Type) (s1 s2: seq a) = f:smap s1 s1 {into_prop f}
+
+let monotonic_prop (#a:_) (#s1 #s2:seq a) (f: smap s1 s2)
+  = forall (i j: seq_index s1). i < j ==> f i < f j
+
+let mono_smap (#a:_) (s1 s2: seq a) = f:smap s1 s2 {monotonic_prop f}
+
+let monotonic_implies_into (#a:_) (#s1 #s2: seq a) (f: smap s1 s2)
+  : Lemma (ensures (monotonic_prop f ==> into_prop f))
+  = ()
+
+val monotonic_bijection_implies_equal (#a:_) (s1 s2: seq a)
+  (f12: mono_smap s1 s2)
+  (f21: mono_smap s2 s1)
+  : Lemma (ensures (s1 == s2))
